Infinite case for interrupt.

lunarlander_sl/ext2/BigStepContinuous.thy
@@ -98,7 +98,7 @@ proof -
   \<comment> \<open>The key result is to show that, for any other solution satisfying
       the ODE, it must be equal to the solution given by d, p.\<close>
   have main:
-    "d2 = d s \<and> p s (d s) = p2 d2 \<and> (\<forall>\<tau>\<in>{0..d s}. p s \<tau> = p2 \<tau>) \<and>
+    "d2 = d s \<and> p s (d s) = p2 d2 \<and>
      WaitBlock (d s) (\<lambda>t\<in>{0..d s}. updr s (p s t)) = WaitBlock d2 (\<lambda>t\<in>{0..d2}. updr s (p2 t))"
     if cond: "b s" "0 < d2"
       "ODEsol ode p2 d2"
@@ -152,7 +152,7 @@ proof -
       using s8 by (simp add: s0 less_eq_real_def)
     have s10: "WaitBlock (d s) (\<lambda>t\<in>{0..d s}. updr s (p s t)) = WaitBlock d2 (\<lambda>t\<in>{0..d2}. updr s (p2 t))"
       using s7 s8 by fastforce
-    show ?thesis using s7 s8 s9 s10 by auto
+    show ?thesis using s7 s9 s10 by auto
   qed
   show ?thesis
     unfolding entails_def apply auto
@@ -170,11 +170,10 @@ proof -
           by (auto simp add: pre(5) rpart.simps updr.simps)
         have a: "d' = d s0"
               "p s0 (d s0) = p' d'"
-              "(\<forall>\<tau>\<in>{0..d s0}. p s0 \<tau> = p' \<tau>)"
               "WaitBlock (d s0) (\<lambda>t\<in>{0..d s0}. updr s0 (p s0 t)) = WaitBlock d' (\<lambda>t\<in>{0..d'}. updr s0 (p' t))"
           using main[of s0 d' p', OF \<open>b s0\<close> pre(2,4,6,7,5)] by auto
         show ?thesis
-          unfolding a(4)[symmetric]
+          unfolding a(3)[symmetric]
           apply (rule wait_sol_c.intros(1))
           using pre(2,3) a(1,2) by auto
       qed
@@ -295,35 +294,6 @@ inductive interrupt_c :: "ODE \<Rightarrow> 'a eform \<Rightarrow> rdy_info \<Ri
    (\<forall>t. 0 \<le> t \<and> t < d \<longrightarrow> b (updr s0 (p t))) \<Longrightarrow>
    interrupt_c ode b rdy P specs s0 s (WaitBlock d (\<lambda>\<tau>\<in>{0..d}. updr s0 (p \<tau>)) rdy # OutBlock ch (e (updr s0 (p d))) # tr)"
 
-text \<open>Special case of one receive communication\<close>
-inductive ode_in_c :: "ODE \<Rightarrow> 'a eform \<Rightarrow> cname \<Rightarrow> rdy_info \<Rightarrow> 'a assn2 \<Rightarrow> (real \<Rightarrow> real \<Rightarrow> 'a assn2) \<Rightarrow> 'a assn2" where
-  "\<not>b s0 \<Longrightarrow> P s0 s tr \<Longrightarrow> ode_in_c ode b ch rdy P Q s0 s tr"
-| "0 < d \<Longrightarrow> P (updr s0 (p d)) s tr \<Longrightarrow> ODEsol ode p d \<Longrightarrow>
-   p 0 = rpart s0 \<Longrightarrow>
-   (\<forall>t. 0 \<le> t \<and> t < d \<longrightarrow> b (updr s0 (p t))) \<Longrightarrow>
-   \<not>b (updr s0 (p d)) \<Longrightarrow>
-   ode_in_c ode b ch rdy P Q s0 s (WaitBlock d (\<lambda>\<tau>\<in>{0..d}. updr s0 (p \<tau>)) rdy # tr)"
-| "Q 0 v s0 s tr \<Longrightarrow> ode_in_c ode b ch rdy P Q s0 s (InBlock ch v # tr)"
-| "0 < d \<Longrightarrow> Q d v (updr s0 (p d)) s tr \<Longrightarrow> ODEsol ode p d \<Longrightarrow>
-   p 0 = rpart s0 \<Longrightarrow>
-   (\<forall>t. 0 \<le> t \<and> t < d \<longrightarrow> b (updr s0 (p t))) \<Longrightarrow>
-   ode_in_c ode b ch rdy P Q s0 s (WaitBlock d (\<lambda>\<tau>\<in>{0..d}. updr s0 (p \<tau>)) rdy # InBlock ch v # tr)"
-
-text \<open>Special case of one send communication\<close>
-inductive ode_out_c :: "ODE \<Rightarrow> 'a eform \<Rightarrow> cname \<Rightarrow> rdy_info \<Rightarrow> ('a estate \<Rightarrow> real) \<Rightarrow> 'a assn2 \<Rightarrow> (real \<Rightarrow> 'a assn2) \<Rightarrow> 'a assn2" where
-  "\<not>b s0 \<Longrightarrow> P s0 s tr \<Longrightarrow> ode_out_c ode b ch rdy e P Q s0 s tr"
-| "0 < d \<Longrightarrow> P (updr s0 (p d)) s tr \<Longrightarrow> ODEsol ode p d \<Longrightarrow>
-   p 0 = rpart s0 \<Longrightarrow>
-   (\<forall>t. 0 \<le> t \<and> t < d \<longrightarrow> b (updr s0 (p t))) \<Longrightarrow>
-   \<not>b (updr s0 (p d)) \<Longrightarrow>
-   ode_out_c ode b ch rdy e P Q s0 s (WaitBlock d (\<lambda>\<tau>\<in>{0..d}. updr s0 (p \<tau>)) rdy # tr)"
-| "Q 0 s0 s tr \<Longrightarrow> ode_out_c ode b ch rdy e P Q s0 s (OutBlock ch (e s0) # tr)"
-| "0 < d \<Longrightarrow> Q d (updr s0 (p d)) s tr \<Longrightarrow> ODEsol ode p d \<Longrightarrow>
-   p 0 = rpart s0 \<Longrightarrow>
-   (\<forall>t. 0 \<le> t \<and> t < d \<longrightarrow> b (updr s0 (p t))) \<Longrightarrow>
-   ode_out_c ode b ch rdy e P Q s0 s (WaitBlock d (\<lambda>\<tau>\<in>{0..d}. updr s0 (p \<tau>)) rdy # OutBlock ch (e s0) # tr)"
-
-
 text \<open>Hoare rules for interrupt\<close>
 
 inductive spec_of_es :: "'a comm \<times> 'a proc \<Rightarrow> 'a comm_spec \<Rightarrow> bool" where
@@ -425,7 +395,6 @@ inductive interrupt_sol_c :: "('a estate \<Rightarrow> real \<Rightarrow> state)
    0 < d' \<Longrightarrow> d' \<le> d s0 \<Longrightarrow> Q d' s0 s tr \<Longrightarrow>
    interrupt_sol_c p d rdy P specs s0 s (WaitBlock d' (\<lambda>\<tau>\<in>{0..d'}. updr s0 (p s0 \<tau>)) rdy # OutBlock ch (e (updr s0 (p s0 d'))) # tr)"
 
-
 lemma interrupt_c_unique:
   assumes
     "paramODEsol ode b p d"
@@ -438,7 +407,7 @@ proof -
   \<comment> \<open>The key result is to show that, for any other solution satisfying
       the ODE, it must be equal to the solution given by d, p.\<close>
   have main:
-    "d2 = d s \<and> p s (d s) = p2 d2 \<and> (\<forall>\<tau>\<in>{0..d s}. p s \<tau> = p2 \<tau>) \<and>
+    "d2 = d s \<and> p s (d s) = p2 d2 \<and>
      WaitBlock (d s) (\<lambda>t\<in>{0..d s}. updr s (p s t)) = WaitBlock d2 (\<lambda>t\<in>{0..d2}. updr s (p2 t))"
     if cond: "b s" "0 < d2"
       "ODEsol ode p2 d2"
@@ -492,10 +461,10 @@ proof -
       using s8 by (simp add: s0 less_eq_real_def)
     have s10: "WaitBlock (d s) (\<lambda>t\<in>{0..d s}. updr s (p s t)) = WaitBlock d2 (\<lambda>t\<in>{0..d2}. updr s (p2 t))"
       using s7 s8 by fastforce
-    show ?thesis using s7 s8 s9 s10 by auto
+    show ?thesis using s7 s9 s10 by auto
   qed
   have main2:
-    "d2 \<le> d s \<and> p s d2 = p2 d2 \<and> (\<forall>\<tau>\<in>{0..d2}. p s \<tau> = p2 \<tau>) \<and>
+    "d2 \<le> d s \<and> p s d2 = p2 d2 \<and>
      WaitBlock d2 (\<lambda>t\<in>{0..d2}. updr s (p s t)) = WaitBlock d2 (\<lambda>t\<in>{0..d2}. updr s (p2 t))"
     if cond: "b s" "0 < d2"
       "ODEsol ode p2 d2"
@@ -538,7 +507,7 @@ proof -
       using s8 that(2) by fastforce
     have s10: "WaitBlock d2 (\<lambda>t\<in>{0..d2}. updr s (p s t)) = WaitBlock d2 (\<lambda>t\<in>{0..d2}. updr s (p2 t))"
       using s7 s8 by fastforce
-    show ?thesis using s6 s8 s9 s10 by auto
+    show ?thesis using s6 s9 s10 by auto
   qed
   have p0: "p s0 0 = rpart s0"
     using paramODEsolD2[OF assms(1)] by auto
@@ -563,11 +532,10 @@ proof -
           by (auto simp add: pre(5) rpart.simps updr.simps)
         have a: "d' = d s0"
               "p s0 (d s0) = p' d'"
-              "(\<forall>\<tau>\<in>{0..d s0}. p s0 \<tau> = p' \<tau>)"
               "WaitBlock (d s0) (\<lambda>t\<in>{0..d s0}. updr s0 (p s0 t)) = WaitBlock d' (\<lambda>t\<in>{0..d'}. updr s0 (p' t))"
           using main[of s0 d' p', OF \<open>b s0\<close> pre(2,4,6,7,5)] by auto
         show ?thesis
-          unfolding a(4)[symmetric]
+          unfolding a(3)[symmetric]
           apply (rule interrupt_sol_c.intros(1))
           using pre(2,3) a(1,2) by auto
       qed
@@ -590,14 +558,13 @@ proof -
           by (auto simp add: pre rpart.simps updr.simps)
         have a: "d' \<le> d s0"
               "p s0 d' = p' d'"
-              "(\<forall>\<tau>\<in>{0..d'}. p s0 \<tau> = p' \<tau>)"
               "WaitBlock d' (\<lambda>t\<in>{0..d'}. updr s0 (p s0 t)) = WaitBlock d' (\<lambda>t\<in>{0..d'}. updr s0 (p' t))"
           using main2[of s0 d' p', OF \<open>b s0\<close> pre(4,6,8,7)] by auto
         let ?Q' = "\<lambda>d v s0. Q (updr s0 ((p s0 d)(var := v)))"
         have Q: "?specs2 ! i = InSpec2 ch ?Q'"
           using speci[OF pre(2)] unfolding pre(3) by auto
         show ?thesis
-          unfolding a(4)[symmetric]
+          unfolding a(3)[symmetric]
           apply (rule interrupt_sol_c.intros(4)[of i _ _ ?Q'])
           using pre(2,3,4,5) a(1,2) Q length by auto
       qed
@@ -620,17 +587,363 @@ proof -
           by (auto simp add: pre rpart.simps updr.simps)
         have a: "d' \<le> d s0"
               "p s0 d' = p' d'"
-              "(\<forall>\<tau>\<in>{0..d'}. p s0 \<tau> = p' \<tau>)"
               "WaitBlock d' (\<lambda>t\<in>{0..d'}. updr s0 (p s0 t)) = WaitBlock d' (\<lambda>t\<in>{0..d'}. updr s0 (p' t))"
           using main2[of s0 d' p', OF \<open>b s0\<close> pre(4,6,8,7)] by auto
         let ?Q' = "\<lambda>d s0. Q (updr s0 (p s0 d))"
         have Q: "?specs2 ! i = OutSpec2 ch e ?Q'"
           using speci[OF pre(2)] unfolding pre(3) by auto
         show ?thesis
-          unfolding a(4)[symmetric] a(2)[symmetric]
+          unfolding a(3)[symmetric] a(2)[symmetric]
           apply (rule interrupt_sol_c.intros(6)[of i _ _ _ ?Q'])
           using pre(2,3,4,5) a(1,2) Q length by auto
       qed
+      done
+    done
+qed
+
+lemma spec_of_interrupt_unique:
+  assumes
+    "paramODEsol ode b p d"
+    "local_lipschitz {- 1<..} UNIV (\<lambda>(t::real) v. ODE2Vec ode (vec2state v))"
+    "length es = length specs"
+    "\<forall>i. i < length es \<longrightarrow> spec_of_es (es ! i) (specs ! i)"
+  shows
+    "spec_of (Interrupt ode b es)
+             (interrupt_sol_c p d (rdy_of_echoice es)
+                              (\<lambda>s. if d s > 0 then init (updr s (p s (d s))) else init s)
+                              (map (spec2_of p) specs))"
+  apply (rule spec_of_post)
+   apply (rule spec_of_interrupt[OF assms(3,4)]) apply auto
+  apply (rule entails_trans)
+   apply (rule interrupt_c_unique[OF assms(1,2)])
+  by (rule entails_triv)
+
+inductive spec2_entails :: "'a comm_spec2 \<Rightarrow> 'a comm_spec2 \<Rightarrow> bool" where
+  "(\<And>d v s0. P1 d v s0 \<Longrightarrow>\<^sub>A P2 d v s0) \<Longrightarrow> spec2_entails (InSpec2 ch P1) (InSpec2 ch P2)"
+| "(\<And>d s0. Q1 d s0 \<Longrightarrow>\<^sub>A Q2 d s0) \<Longrightarrow> spec2_entails (OutSpec2 ch e Q1) (OutSpec2 ch e Q2)"
+
+inductive_cases spec2_entails_inE: "spec2_entails (InSpec2 ch P1) spec2"
+inductive_cases spec2_entails_outE: "spec2_entails (OutSpec2 ch e Q1) spec2"
+
+lemma interrupt_sol_mono:
+  assumes "\<And>s0. P s0 \<Longrightarrow>\<^sub>A P2 s0"
+    and "length specs = length specs2"
+    and "\<And>i. i < length specs \<Longrightarrow> spec2_entails (specs ! i) (specs2 ! i)"
+  shows "interrupt_sol_c p d rdy P specs s0 \<Longrightarrow>\<^sub>A interrupt_sol_c p d rdy P2 specs2 s0"
+  unfolding entails_def apply auto
+  subgoal for s tr
+    apply (induct rule: interrupt_sol_c.cases) apply auto
+    subgoal for tr' a b
+      apply (rule interrupt_sol_c.intros(1))
+      using assms(1) unfolding entails_def by auto
+    subgoal for a b
+      apply (rule interrupt_sol_c.intros(2))
+      using assms(1) unfolding entails_def by auto
+    subgoal for i ch Q v tr' a b
+      using assms(3)[of i] apply simp
+      apply (elim spec2_entails_inE)
+      subgoal for Q2
+        apply (rule interrupt_sol_c.intros(3)[of i _ _ Q2])
+        using assms(2) unfolding entails_def by auto
+      done
+    subgoal for i ch Q d' v tr' a b
+      using assms(3)[of i] apply simp
+      apply (elim spec2_entails_inE)
+      subgoal for Q2
+        apply (rule interrupt_sol_c.intros(4)[of i _ _ Q2])
+        using assms(2) unfolding entails_def by auto
+      done
+    subgoal for i ch e Q tr' a b
+      using assms(3)[of i] apply simp
+      apply (elim spec2_entails_outE)
+      subgoal for Q2
+        apply (rule interrupt_sol_c.intros(5)[of i _ _ _ Q2])
+        using assms(2) unfolding entails_def by auto
+      done
+    subgoal for i ch e Q d' tr' a b
+      using assms(3)[of i] apply simp
+      apply (elim spec2_entails_outE)
+      subgoal for Q2
+        apply (rule interrupt_sol_c.intros(6)[of i _ _ _ Q2])
+        using assms(2) unfolding entails_def by auto
+      done
+    done
+  done
+
+lemma test2:
+  "spec_of (Interrupt (ODE ((\<lambda>_ _. 0)(X := (\<lambda>_. 1)))) (\<lambda>s. val s X < 1)
+                      [(dh[?]Y, Skip)])
+           (interrupt_sol_c (\<lambda>s0 t. (rpart s0)(X := val s0 X + t)) (\<lambda>s0. 1 - val s0 X)
+                            ({}, {dh}) (\<lambda>s. if val s X < 1 then init (upd s X 1) else init s)
+                            [InSpec2 dh (\<lambda>d v s. init (upd (upd s X (val s X + d)) Y v))])"
+proof -
+  have 1: "paramODEsol (ODE ((\<lambda>_ _. 0)(X := \<lambda>_. 1))) (\<lambda>s. val s X < 1)
+                       (\<lambda>s0 t. (rpart s0)(X := val s0 X + t)) (\<lambda>s0. 1 - val s0 X)"
+    unfolding paramODEsol_def apply clarify
+    subgoal for s
+      apply (rule conjI)
+      subgoal apply (cases s)
+        by (auto simp add: rpart.simps val.simps)
+      apply (cases "val s X < 1")
+      subgoal apply auto
+        subgoal
+          unfolding ODEsol_def solves_ode_def has_vderiv_on_def
+          apply auto
+          apply (rule exI[where x="1"])
+          apply auto
+          apply (rule has_vector_derivative_projI)
+          apply (auto simp add: state2vec_def)
+          apply (rule has_vector_derivative_eq_rhs)
+           apply (auto intro!: derivative_intros)[1]
+          by simp
+        subgoal for t
+          apply (cases s) by (auto simp add: updr.simps val.simps)
+        subgoal 
+          apply (cases s) by (auto simp add: updr.simps val.simps)
+        done
+      subgoal by auto
+      done
+    done
+  have 2: "local_lipschitz {- 1<..} UNIV (\<lambda>t v. ODE2Vec (ODE ((\<lambda>_ _. 0)(X := \<lambda>_. 1))) (vec2state v))"
+  proof -
+    have eq: "(\<chi> a. (if a = X then \<lambda>_. 1 else (\<lambda>_. 0)) (($) v)) = (\<chi> a. if a = X then 1 else 0)" for v::vec
+      by auto
+    show ?thesis
+      unfolding fun_upd_def vec2state_def
+      apply (auto simp add: state2vec_def eq)
+      by (rule local_lipschitz_constI)
+  qed
+  let ?specs = "[InSpec dh Y init]"
+  show ?thesis
+    apply (rule spec_of_post)
+     apply (rule spec_of_interrupt_unique[where specs="?specs"])
+        apply (rule 1) apply (rule 2)
+      apply auto apply (rule spec_of_es.intros)
+     apply (rule spec_of_skip)
+    subgoal for s0
+      apply (rule interrupt_sol_mono)
+      subgoal for s0
+        apply (cases s0) apply (auto simp add: updr.simps upd.simps rpart.simps)
+        by (rule entails_triv)+
+      subgoal by auto
+      subgoal for i
+        apply auto apply (intro spec2_entails.intros)
+        subgoal for d v s0
+          apply (cases s0) apply (auto simp add: updr.simps upd.simps rpart.simps)
+          by (rule entails_triv)
+        done
+      done
+    done
+qed
+
+inductive interrupt_solInf_c :: "('a estate \<Rightarrow> real \<Rightarrow> state) \<Rightarrow> rdy_info \<Rightarrow>
+  'a comm_spec2 list \<Rightarrow> 'a assn2" where
+  "i < length specs \<Longrightarrow> specs ! i = InSpec2 ch Q \<Longrightarrow>
+   Q 0 v s0 s tr \<Longrightarrow> interrupt_solInf_c p rdy specs s0 s (InBlock ch v # tr)"
+| "i < length specs \<Longrightarrow> specs ! i = InSpec2 ch Q \<Longrightarrow>
+   0 < d \<Longrightarrow> Q d v s0 s tr \<Longrightarrow>
+   interrupt_solInf_c p rdy specs s0 s (WaitBlock d (\<lambda>\<tau>\<in>{0..d}. updr s0 (p s0 \<tau>)) rdy # InBlock ch v # tr)"
+| "i < length specs \<Longrightarrow> specs ! i = OutSpec2 ch e Q \<Longrightarrow>
+   Q 0 s0 s tr \<Longrightarrow> interrupt_solInf_c p rdy specs s0 s (OutBlock ch (e s0) # tr)"
+| "i < length specs \<Longrightarrow> specs ! i = OutSpec2 ch e Q \<Longrightarrow>
+   0 < d \<Longrightarrow> Q d s0 s tr \<Longrightarrow>
+   interrupt_solInf_c p rdy specs s0 s (WaitBlock d (\<lambda>\<tau>\<in>{0..d}. updr s0 (p s0 \<tau>)) rdy # OutBlock ch (e (updr s0 (p s0 d))) # tr)"
+
+definition paramODEsolInf :: "ODE \<Rightarrow> ('a estate \<Rightarrow> real \<Rightarrow> state) \<Rightarrow> bool" where
+  "paramODEsolInf ode p \<longleftrightarrow>
+    (\<forall>s. p s 0 = rpart s \<and> ODEsolInf ode (p s))"
+
+lemma interrupt_inf_c_unique:
+  assumes
+    "paramODEsolInf ode p"
+    "local_lipschitz {- 1<..} UNIV (\<lambda>(t::real) v. ODE2Vec ode (vec2state v))"
+  shows
+    "interrupt_c ode (\<lambda>_. True) rdy P specs s0 \<Longrightarrow>\<^sub>A
+     interrupt_solInf_c p rdy (map (spec2_of p) specs) s0"
+proof -
+  have main:
+    "p s d2 = p2 d2 \<and>
+     WaitBlock d2 (\<lambda>t\<in>{0..d2}. updr s (p s t)) = WaitBlock d2 (\<lambda>t\<in>{0..d2}. updr s (p2 t))"
+    if cond: "0 < d2" "ODEsol ode p2 d2" "p2 0 = rpart s" for s p2 d2
+  proof -
+    interpret loc:ll_on_open_it "{-1<..}"
+      "\<lambda>t v. ODE2Vec ode (vec2state v)" UNIV 0
+      apply standard
+      using assms(2) by auto
+    have s1: "((\<lambda>t. state2vec (p s t)) solves_ode ((\<lambda>t v. ODE2Vec ode (vec2state v)))) {0..} UNIV"
+      using assms(1) ODEsolInf_old unfolding paramODEsolInf_def solves_ode_def by auto
+    have s2: "(loc.flow 0 (state2vec (rpart s))) t = (\<lambda>t. state2vec (p s t)) t" if "t \<in> {0..d2}" for t
+      apply (rule loc.maximal_existence_flow(2)[OF s1])
+      using that assms(1) unfolding paramODEsolInf_def
+      by (auto simp add: state2vec_def)
+    have s3: "((\<lambda>t. state2vec (p2 t)) solves_ode ((\<lambda>t v. ODE2Vec ode (vec2state v)))) {0..d2} UNIV"
+      using cond(2) ODEsol_old unfolding ODEsol_def solves_ode_def by auto
+    have s4: "loc.flow 0 (state2vec (rpart s)) t = state2vec (p2 t)" if "t\<in>{0..d2}" for t
+      apply (rule loc.maximal_existence_flow(2)[OF s3])
+      using cond that by auto
+    have s7: "t\<in>{0..d2} \<Longrightarrow> loc.flow 0 (state2vec (rpart s)) t = state2vec (p s t)" for t
+      using s2 by auto
+    have s8: "t\<in>{0..d2} \<Longrightarrow> p2 t = p s t" for t
+      using s7 s4 by (metis vec_state_map1)
+    have s9: "p s d2 = p2 d2"
+      using s8 that(1) by fastforce
+    have s10: "WaitBlock d2 (\<lambda>t\<in>{0..d2}. updr s (p s t)) = WaitBlock d2 (\<lambda>t\<in>{0..d2}. updr s (p2 t))"
+      using s7 s8 by fastforce
+    show ?thesis using s8 s9 s10 by auto
+  qed
+  have p0: "p s0 0 = rpart s0"
+    using assms(1) unfolding paramODEsolInf_def by auto
+  let ?specs2 = "map (spec2_of p) specs"
+  have length: "length ?specs2 = length specs"
+    by auto
+  have speci: "?specs2 ! i = spec2_of p (specs ! i)" if "i < length specs" for i
+    using that by auto
+  show ?thesis
+    unfolding entails_def apply auto
+    subgoal for s tr
+      apply (auto simp add: interrupt_c.simps)
+      subgoal premises pre for i ch var Q v tr'
+      proof -
+        let ?Q' = "\<lambda>d v s0. Q (updr s0 ((p s0 d)(var := v)))"
+        show ?thesis
+          apply (rule interrupt_solInf_c.intros(1)[of i _ _ ?Q'])
+          using pre length p0 apply auto
+          apply (cases s0) by (auto simp add: updr.simps rpart.simps upd.simps)
+      qed
+      subgoal premises pre for i ch var Q d p2 v tr'
+      proof -
+        have a: "p s0 d = p2 d"
+             "WaitBlock d (\<lambda>t\<in>{0..d}. updr s0 (p s0 t)) = WaitBlock d (\<lambda>t\<in>{0..d}. updr s0 (p2 t))"
+          using main[of d p2 s0, OF pre(4,6,7)] by auto
+        let ?Q' = "\<lambda>d v s0. Q (updr s0 ((p s0 d)(var := v)))"
+        show ?thesis
+          unfolding a(2)[symmetric]
+          apply (rule interrupt_solInf_c.intros(2)[of i _ _ ?Q'])
+          using pre a length by auto
+      qed
+      subgoal premises pre for i ch e Q tr'
+      proof -
+        let ?Q' = "\<lambda>d s0. Q (updr s0 (p s0 d))"
+        show ?thesis
+          apply (rule interrupt_solInf_c.intros(3)[of i _ _ _ ?Q'])
+          using pre length p0 apply auto
+          apply (cases s0) by (auto simp add: updr.simps rpart.simps)
+      qed
+      subgoal premises pre for i ch e Q d p2 tr'
+      proof -
+        have a: "p s0 d = p2 d"
+             "WaitBlock d (\<lambda>t\<in>{0..d}. updr s0 (p s0 t)) = WaitBlock d (\<lambda>t\<in>{0..d}. updr s0 (p2 t))"
+          using main[of d p2 s0, OF pre(4,6,7)] by auto
+        let ?Q' = "\<lambda>d s0. Q (updr s0 (p s0 d))"
+        show ?thesis
+          unfolding a(2)[symmetric] a(1)[symmetric]
+          apply (rule interrupt_solInf_c.intros(4)[of i _ _ _ ?Q'])
+          using pre length a(1) by auto
+      qed
+      done
+    done
+qed
+
+lemma spec_of_interrupt_inf_unique:
+  assumes
+    "paramODEsolInf ode p"
+    "local_lipschitz {- 1<..} UNIV (\<lambda>(t::real) v. ODE2Vec ode (vec2state v))"
+    "length es = length specs"
+    "\<forall>i. i < length es \<longrightarrow> spec_of_es (es ! i) (specs ! i)"
+  shows
+    "spec_of (Interrupt ode (\<lambda>_. True) es)
+             (interrupt_solInf_c p (rdy_of_echoice es) (map (spec2_of p) specs))"
+  apply (rule spec_of_post)
+   apply (rule spec_of_interrupt[OF assms(3,4)]) apply auto
+  apply (rule entails_trans)
+   apply (rule interrupt_inf_c_unique[OF assms(1,2)])
+  by (rule entails_triv)
+
+lemma interrupt_solInf_mono:
+  assumes "length specs = length specs2"
+    and "\<And>i. i < length specs \<Longrightarrow> spec2_entails (specs ! i) (specs2 ! i)"
+  shows "interrupt_solInf_c p rdy specs s0 \<Longrightarrow>\<^sub>A interrupt_solInf_c p rdy specs2 s0"
+  unfolding entails_def apply auto
+  subgoal for s tr
+    apply (induct rule: interrupt_solInf_c.cases) apply auto
+    subgoal for i ch Q v tr' a b
+      using assms(2)[of i] apply simp
+      apply (elim spec2_entails_inE)
+      subgoal for Q2
+        apply (rule interrupt_solInf_c.intros(1)[of i _ _ Q2])
+        using assms(1) unfolding entails_def by auto
+      done
+    subgoal for i ch Q d' v tr' a b
+      using assms(2)[of i] apply simp
+      apply (elim spec2_entails_inE)
+      subgoal for Q2
+        apply (rule interrupt_solInf_c.intros(2)[of i _ _ Q2])
+        using assms(1) unfolding entails_def by auto
+      done
+    subgoal for i ch e Q tr' a b
+      using assms(2)[of i] apply simp
+      apply (elim spec2_entails_outE)
+      subgoal for Q2
+        apply (rule interrupt_solInf_c.intros(3)[of i _ _ _ Q2])
+        using assms(1) unfolding entails_def by auto
+      done
+    subgoal for i ch E Q d tr' a b
+      using assms(2)[of i] apply simp
+      apply (elim spec2_entails_outE)
+      subgoal for Q2
+        apply (rule interrupt_solInf_c.intros(4)[of i _ _ _ Q2])
+        using assms(1) unfolding entails_def by auto
+      done
+    done
+  done
+
+lemma test3:
+  "spec_of (Interrupt (ODE ((\<lambda>_ _. 0)(X := (\<lambda>_. 1)))) (\<lambda>_. True)
+                      [(dh[?]Y, Skip)])
+           (interrupt_solInf_c (\<lambda>s0 t. (rpart s0)(X := val s0 X + t))
+                               ({}, {dh})
+                               [InSpec2 dh (\<lambda>d v s. init (upd (upd s X (val s X + d)) Y v))])"
+proof -
+  have 1: "paramODEsolInf (ODE ((\<lambda>_ _. 0)(X := \<lambda>_. 1)))
+                       (\<lambda>s0 t. (rpart s0)(X := val s0 X + t))"
+    unfolding paramODEsolInf_def apply clarify
+    subgoal for s
+      apply (rule conjI)
+      subgoal apply (cases s)
+        by (auto simp add: rpart.simps val.simps)
+      unfolding ODEsolInf_def solves_ode_def has_vderiv_on_def
+      apply auto
+      apply (rule exI[where x="1"])
+      apply auto
+      apply (rule has_vector_derivative_projI)
+      apply (auto simp add: state2vec_def)
+      apply (rule has_vector_derivative_eq_rhs)
+       apply (auto intro!: derivative_intros)[1]
+      by simp
+    done
+  have 2: "local_lipschitz {- 1<..} UNIV (\<lambda>t v. ODE2Vec (ODE ((\<lambda>_ _. 0)(X := \<lambda>_. 1))) (vec2state v))"
+  proof -
+    have eq: "(\<chi> a. (if a = X then \<lambda>_. 1 else (\<lambda>_. 0)) (($) v)) = (\<chi> a. if a = X then 1 else 0)" for v::vec
+      by auto
+    show ?thesis
+      unfolding fun_upd_def vec2state_def
+      apply (auto simp add: state2vec_def eq)
+      by (rule local_lipschitz_constI)
+  qed
+  let ?specs = "[InSpec dh Y init]"
+  show ?thesis
+    apply (rule spec_of_post)
+     apply (rule spec_of_interrupt_inf_unique[where specs="?specs"])
+        apply (rule 1) apply (rule 2)
+      apply auto apply (rule spec_of_es.intros)
+     apply (rule spec_of_skip)
+    subgoal for s0
+      apply (rule interrupt_solInf_mono)
+       apply auto
+      apply (intro spec2_entails.intros)
+      subgoal for d v s0
+        apply (cases s0) apply (auto simp add: updr.simps rpart.simps val.simps upd.simps)
+        by (rule entails_triv)
       done
     done
 qed
